Cleaning, complete memory refinement

AbstractMachine.v
@@ -1,12 +1,13 @@
+Require Import Instructions.
 Require Import AbstractRegister.
 Require Import AbstractMemory.
+Require Import MemoryR.
 Require Import MachineInt.
-
-Definition PC := word.
+Require Import Coqlib.
 
 Inductive Flag : Set :=
   | C : Flag
-  | Z : Flag
+  | Zero : Flag
   | I : Flag
   | D : Flag
   | B : Flag
@@ -24,62 +25,108 @@ Record Status : Set :=
   SF : bool
 }.
 
-(*Definition setFlag (S: Status) (f: Flag): Status :=
+Definition setFlag (S: Status) (f: Flag): Status :=
   match f with
-  | Si => mkState S.() S.() S.() S.() S.() S.() true
-  | V => mkState S.() S.() S.() S.() S.() true S.()
-  | B => mkState S.() S.() S.() S.() S.() S.() true
-  | D => mkState S.() S.() S.() S.() S.() S.() true
-  | I => mkState S.() S.() S.() S.() S.() S.() true
-  | Z => mkState S.() S.() S.() S.() S.() S.() true
-  | C => mkState S.() S.() S.() S.() S.() S.() true.
-  end.*)
-
-(*Definition clearFlag (S: Status) (f: Flag): Status :=
-  match f with
-  | Si => 
-  | V => 
-  | B => 
-  | D => 
-  | I => 
-  | Z => 
-  | C => 
-  end.*)
-
-Definition State := (AbstractRegister.RegF * AbstractMemory.Mem * PC * Status)%type.
-
-Definition _R (S : State) :=
-  match S with
-    | (R, _, _, _) => R
+  | Si => mkState S.(CF) S.(ZF) S.(InF) S.(DF) S.(BF) S.(VF) true
+  | V => mkState S.(CF) S.(ZF) S.(InF) S.(DF) S.(BF) true S.(SF)
+  | B => mkState S.(CF) S.(ZF) S.(InF) S.(DF) true S.(VF) S.(SF)
+  | D => mkState S.(CF) S.(ZF) S.(InF) true S.(BF) S.(VF) S.(SF)
+  | I => mkState S.(CF) S.(ZF) true S.(DF) S.(BF) S.(VF) S.(SF) 
+  | Zero => mkState S.(CF) true S.(InF) S.(DF) S.(BF) S.(VF) S.(SF) 
+  | C => mkState true S.(ZF) S.(InF) S.(DF) S.(BF) S.(VF) S.(SF)
   end.
 
-Definition _M (S : State) :=
-  match S with
-    | (_, M, _, _) => M
+Definition clearFlag (S: Status) (f: Flag): Status :=
+  match f with
+  | Si => mkState S.(CF) S.(ZF) S.(InF) S.(DF) S.(BF) S.(VF) false
+  | V => mkState S.(CF) S.(ZF) S.(InF) S.(DF) S.(BF) false S.(SF)
+  | B => mkState S.(CF) S.(ZF) S.(InF) S.(DF) false S.(VF) S.(SF)
+  | D => mkState S.(CF) S.(ZF) S.(InF) false S.(BF) S.(VF) S.(SF)
+  | I => mkState S.(CF) S.(ZF) false S.(DF) S.(BF) S.(VF) S.(SF) 
+  | Zero => mkState S.(CF) false S.(InF) S.(DF) S.(BF) S.(VF) S.(SF) 
+  | C => mkState false S.(ZF) S.(InF) S.(DF) S.(BF) S.(VF) S.(SF)
   end.
 
-Definition _PC (S : State) :=
+Definition State := (AbstractRegister.RegF * AbstractMemory.Mem * word * Status)%type.
+
+Definition R (S : State) :=
+  match S with
+    | (r, _, _, _) => r
+  end.
+
+Definition M (S : State) :=
+  match S with
+    | (_, m, _, _) => m
+  end.
+
+Definition PC (S : State) :=
   match S with
     | (_, _, pc, _) => pc
   end.
 
-Definition _ST (S : State) :=
+Definition ST (S : State) :=
   match S with
     | (_, _, _, st) => st
   end.
 
-Module AbstractMachine.
+Definition nextinstr (S: State) : State :=
+(R S, M S, (Word.repr (Word.intval (PC S) + 1)), ST S).
 
-Module Context.
+Inductive outcome: Type :=
+  | Next: State -> outcome
+  | Stuck: outcome.
 
-End Context.
+Definition exec_load (a: nat) (dest: AbstractRegister.Reg8) (S: State) :=
+  match MemoryR.Load.load8 (M S) a with
+  | MemoryR.Safe v => Next (nextinstr (AbstractRegister.SetRegister.setReg8 (R S) dest v, M S, PC S, ST S))
+  | _ => Stuck
+  end.
 
-Definition Inv_1 (B: State) : Prop := True.
+Definition exec_store (a: nat) (S: State) (source: AbstractRegister.Reg8) :=
+  match MemoryR.Store.store8 (M S) a (AbstractRegister.GetRegisterValue.getReg8 (R S) source) with
+  | Some m' => Next (nextinstr (R S, m', PC S, ST S))
+  | None => Stuck
+  end.
 
-Module Init.
+Definition exec_load_imm (b: byte) (S : State) (r : AbstractRegister.Reg8) :=
+ Next (nextinstr (AbstractRegister.SetRegister.setReg8 (R S) r b, M S, PC S, ST S)).
 
-Definition Guard : Prop := True.
+Definition exec_instr (i: Instr) (S: State) :=
+  match i with
+    LDA_ir b => exec_load_imm b S A
+  | LDX_ir b => exec_load_imm b S X
+  | LDY_ir b => exec_load_imm b S Y
+  | LDA_mr l => exec_load l A S
+  | LDX_mr l => exec_load l X S
+  | LDY_mr l => exec_load l Y S
+  | STA_rm l => exec_store l S A
+  | STX_rm l => exec_store l S X
+  | STY_rm l => exec_store l S Y
+  | ADC_mr l => Next (S)
+  | SBC_mr l => Next (S)
+  | _ => Next (S)
+end.
 
-End Init.
+Fixpoint find_instr (pos: Z) (code: list Instr) : option Instr :=
+  match code with
+  | nil => None
+  | i :: il => if zeq pos 0 then Some i else find_instr (pos - 1) il
+  end.
 
-End AbstractMachine.
+Fixpoint step (S1 : State) (p: list Instr) : option State :=
+      match find_instr (Word.intval (PC S1)) p with
+        Some i => match exec_instr i S1 with
+                    Next S2 => Some S2
+                    |Stuck => None
+                    end
+        | None => None
+        end.
+
+Fixpoint run (S1 : State) (p: list Instr) (n : nat) : option State :=
+  match n with
+  | 0%nat => Some S1
+  | S n' => match step S1 p with
+              | Some S2 => run S2 p n'
+              | None => None
+              end
+end.
