AbstractMemory.v
@@ -20,34 +20,20 @@ End Init.
 
 Module Store.
 
-(*
-Lemma belong: forall A : Set, forall l1 l2 l3 : list A, forall e : A, forall n : nat,
-app l2 l3 = l1
--> l2 = firstn n l1 -> l3 = skipn n l1
--> (length l2 = n /\ length l3 = (length l1 - n) /\ length l1 >= 0 /\  n < length l1) 
--> replace_at l1 n e = app l2 (e::l3).
-intros A l1 l2 l3 e n.
-simpl.
-intros H1 H2 H3 H4.
+Definition Inv_1 (M: Mem) : Prop := True.
 
-induction l1 as [|x lx].
-+simpl.
-rewrite app_eq_nil in H1.
-inversion H1.
-*)
+Definition store8 (M : Mem) (l : nat) (b : byte) : Mem := 
+match replace_at M l b with 
+| Some M' => M'
+| None => M
+end.
 
-Definition Inv_1 (M: option Mem) : Prop := True.
+Definition action (S : Mem) (l : nat) (b : byte) : Mem := store8 S l b.
 
-Definition store8 (M : Mem) (l : nat) (b : byte) : option Mem := replace_at M l b.
-
-Definition action (S : Mem) (l : nat) (b : byte) : option Mem := store8 S l b.
-
-Lemma PO_Safety: forall S: Mem, forall l: nat, forall b: byte, Init.Guard 4096 -> Guard l -> let S' := action S l b in Inv_1 S'.
+Lemma PO_Safety: forall S: Mem, forall l: nat, forall b: byte, Guard l -> let S' := action S l b in Inv_1 S'.
 intros S l b.
 simpl.
 compute.
-intro.
-rewrite H.
 split.
 Qed.
 
@@ -65,24 +51,23 @@ Definition load8 (M : Mem) (l : nat) : byte :=
 
 Definition action (S : Mem) (l : nat) : byte := load8 S l.
 
-Lemma PO_Safety: forall S: Mem, forall l: nat, Init.Guard 4096 -> Guard l -> let b' := action S l in Inv_1 b'.
+Lemma PO_Safety: forall S: Mem, forall l: nat, Guard l -> let b' := action S l in Inv_1 b'.
 intros S l.
 compute.
-intro H.
-rewrite H.
 split.
 Qed.
 
 End Load.
 
-(*
+
 Lemma load_store_eq_8 :
   forall (M : Mem) (l : nat) (b : byte), Load.load8 (Store.store8 M l b) l = b.
 intros S l b.
 unfold Store.store8.
-unfold Store.replace_at.
+unfold replace_at.
 compute.
 simpl.
-*)
+Admitted.
+
 
 End AbstractMemory.
