Main.v
@@ -1,57 +1,20 @@
-Require Import AbstractMachine.
-Require Import Instructions.
-Require Import AbstractRegister.
-Require Import AbstractMemory.
 Require Import MachineInt.
 Require Import Coqlib.
 Require Import Repeat.
 
-Definition nextinstr (S: State) : State :=
-(_R S, _M S, (Word.repr (Word.intval (_PC S) + 1)), _ST S).
+Require Import Instructions.
+Require Import AbstractRegister.
+Require Import AbstractMachine.
 
-Inductive outcome: Type :=
-  | Next: State -> outcome
-  | Stuck: outcome.
+Definition StartR := AbstractRegister.mkState (Byte.repr 0) (Byte.repr 0) (Byte.repr 0).
 
-Definition exec_load (a: nat) (dest: AbstractRegister.Reg8) (S: State) :=
-  match AbstractMemory.Load.load8 (_M S) a with
-  | v => Next (nextinstr (AbstractRegister.SetRegister.setReg8 (_R S) dest v, _M S, _PC S, _ST S))
-  end.
+Definition StartM := repeat (Byte.repr 0) 4096.
 
-Definition exec_store (a: nat) (S: State) (source: AbstractRegister.Reg8) :=
-  match AbstractMemory.Store.store8 (_M S) a (AbstractRegister.GetRegisterValue.getReg8 (_R S) source) with
-  | Some m' => Next (nextinstr (_R S, m', _PC S, _ST S))
-  | None => Stuck
-  end.
+Definition StartPC := Word.repr 0.
 
-Definition exec_load_imm (b: byte) (S : State) (R : AbstractRegister.Reg8) :=
- Next (nextinstr (AbstractRegister.SetRegister.setReg8 (_R S) R b, _M S, _PC S, _ST S)).
+Definition StartST := AbstractMachine.mkState false false false false false false false.
 
-Definition exec_instr (i: Instr) (S: State) :=
-  match i with
-    LDA_ir b => exec_load_imm b S A
-  | LDX_ir b => exec_load_imm b S X
-  | LDY_ir b => exec_load_imm b S Y
-  | LDA_mr l => exec_load l A S
-  | LDX_mr l => exec_load l X S
-  | LDY_mr l => exec_load l Y S
-  | STA_rm l => exec_store l S A
-  | STX_rm l => exec_store l S X
-  | STY_rm l => exec_store l S Y
-  | ADC_mr l => Next (S)
-  | SBC_mr l => Next (S)
-  | _ => Next (S)
-end.
-
-Definition StartR : AbstractRegister.RegF := AbstractRegister.mkState (Byte.repr 0) (Byte.repr 0) (Byte.repr 0).
-
-Definition StartM : AbstractMemory.Mem := repeat (Byte.repr 0) 4096.
-
-Definition StartPC : word := Word.repr 0.
-
-Definition StartST : Status := AbstractMachine.mkState false false false false false false false.
-
-Definition StartP : State := (StartR, StartM, StartPC, StartST).
+Definition StartP := (StartR, StartM, StartPC, StartST).
 
 Definition prog1 : list Instr :=
   (LDA_ir (Byte.repr 1)) ::
@@ -63,28 +26,20 @@ Definition prog1 : list Instr :=
   (STX_rm 6) ::
   nil.
 
-Fixpoint find_instr (pos: Z) (code: list Instr) : option Instr :=
-  match code with
-  | nil => None
-  | i :: il => if zeq pos 0 then Some i else find_instr (pos - 1) il
-  end.
-
-Fixpoint step (S1 : State) (p: list Instr) : option State :=
-      match find_instr (Word.intval (_PC S1)) p with
-        Some i => match exec_instr i S1 with
-                    Next S2 => Some S2
-                    |Stuck => None
-                    end
-        | None => None
-        end.
-
-Fixpoint run (S1 : State) (p: list Instr) (n : nat) : State :=
-  match n with
-  | 0%nat => S1
-  | S n' => match step S1 p with
-              | Some S2 => run S2 p n'
-              | None => S1
-              end
-end.
-
 Eval compute in run StartP prog1 100.
+
+Definition prog2 : list Instr :=
+  (LDX_ir (Byte.repr 4)) ::
+  (STX_rm 6) ::
+  (LDX_mr 6) ::
+  nil.
+
+Eval compute in run StartP prog2 2.
+
+Definition prog3 : list Instr :=
+  (LDX_ir (Byte.repr 4)) ::
+  (LDX_mr 6) ::
+  (STX_rm 6) ::
+  nil.
+
+Eval compute in run StartP prog3 3.
